icing/CakeMLtoFloVerScript.sml
@@ -11,30 +11,7 @@ open preamble;
 
 val _ = new_theory "CakeMLtoFloVer";
 
-Definition isFloVerExps_def:
-  isFloVerExps [Var x] = T ∧
-  isFloVerExps [App op exps] =
-    (isFloVerExps exps  ∧
-    (case op of
-     | FP_bop _ => LENGTH exps = 2
-     | FP_uop FP_Neg => LENGTH exps = 1
-     | FP_top _ => LENGTH exps = 3
-     | _ =>  F)) ∧
-  isFloVerExps [e] = F ∧
-  isFloVerExps (e1::es) = (isFloVerExps [e1] ∧ isFloVerExps es)
-Termination
-  wf_rel_tac `measure exp6_size`
-End
-
-Definition isFloVerCmd_def:
-  isFloVerCmd (Let so e1 e2) =
-  (case so of
-   | SOME x => isFloVerExps [e1] ∧ isFloVerCmd e2
-   | NONE => F) ∧
-  isFloVerCmd (App op exps) = isFloVerExps [App op exps] ∧
-  isFloVerCmd (Var x) = T ∧
-  isFloVerCmd _ = F
-End
+(** Translation from CakeML AST to FloVer AST **)
 
 Definition fpBopToFloVer_def:
   fpBopToFloVer (FP_Add) = Expressions$Plus ∧
@@ -43,12 +20,14 @@ Definition fpBopToFloVer_def:
   fpBopToFloVer (FP_Div) = Div
 End
 
+Type nameP[pp] = “:(string, string) id # num”;
+
 Definition lookupCMLVar_def:
-  lookupCMLVar n ns = FIND (λ (m,i). n = m) ns
+  lookupCMLVar n (ns:nameP list) = FIND (λ (m,i). n = m) ns
 End
 
 Definition lookupFloVerVar_def:
-  lookupFloVerVar n ns = FIND (λ (m,i). n = i) ns
+  lookupFloVerVar n (ns:nameP list) = FIND (λ (m,i). n = i) ns
 End
 
 Definition appendCMLVar_def:
@@ -58,20 +37,25 @@ Definition appendCMLVar_def:
   | NONE => (n,i)::ns
 End
 
-Definition prepareVars_def:
-  prepareVars [] = SOME ([],[],0:num) ∧
-  prepareVars (v1::vs) =
-    (case prepareVars vs of
-    | NONE => NONE
-    | SOME (ns, ids, freshId)  =>
-    (case (lookupCMLVar (Short v1) ids) of
-     | SOME _ => NONE
-     | NONE => SOME (freshId::ns, appendCMLVar ((Short v1):(string,string) id) freshId ids, freshId+1)))
+(** WAS: prepareVars **)
+Definition getFloVerVarMap_def:
+  getFloVerVarMap ([]:(((string,string) id) list)) = SOME ([],[], 0:num) ∧
+  getFloVerVarMap (v1::vs) =
+  case getFloVerVarMap vs of
+  | NONE => NONE
+  | SOME (ns, ids, freshId) =>
+  case lookupCMLVar v1 ids of
+  | SOME _ => NONE (* Double occurrence of variable *)
+  | NONE =>
+  case v1 of
+  | Short s => SOME (ns++[freshId], appendCMLVar v1 freshId ids, freshId+1)
+  | _ => NONE
 End
 
-Definition prepareGamma_def:
-  prepareGamma [] = FloverMapTree_empty ∧
-  prepareGamma (n1::ns) = FloverMapTree_insert (Var n1) M64 (prepareGamma ns)
+(* WAS: prepareGamma *)
+Definition buildFloVerTypeMap_def:
+  buildFloVerTypeMap [] = FloverMapTree_empty ∧
+  buildFloVerTypeMap (n1::ns) = FloverMapTree_insert (Var n1) M64 (buildFloVerTypeMap ns)
 End
 
 Definition toFloVerConst_def:
@@ -106,6 +90,7 @@ Definition toFloVerExp_def:
     | _, _, _ => NONE)
    | (_, _) => NONE)
   ∧
+  toFloVerExp ids (FpOptimise NoOpt e) = toFloVerExp ids e ∧
   toFloVerExp _ _ = NONE
 End
 
@@ -140,6 +125,7 @@ Definition toFloVerCmd_def:
     (case toFloVerExp ids (Lit l) of
     | NONE => NONE
     | SOME fexp1 => SOME (ids, freshId, Commands$Ret fexp1)) ∧
+  toFloVerCmd ids freshId (FpOptimise NoOpt e) = toFloVerCmd ids freshId e ∧
   toFloVerCmd _ _ _ = NONE
 End
 
@@ -154,6 +140,8 @@ Definition toFloVerEnv_def:
    |SOME (Real r) => SOME r
    |_ => NONE)
 End
+
+(** Translation from FP ops to Real ops **)
 
 Definition getRealCmp_def:
   getRealCmp (FP_Less) = Real_Less ∧
@@ -176,17 +164,18 @@ Definition getRealBop_def:
   getRealBop (FP_Div) = Real_Div
 End
 
-Definition toRealExp_def:
-  toRealExp (Lit (Word64 w)) = Lit (Word64 w) (* RealFromFP added in App case *)∧
-  toRealExp (Lit l) = Lit l ∧
-  toRealExp (Var x) = Var x ∧
-  toRealExp (Raise e) = Raise (toRealExp e) ∧
-  toRealExp (Handle e pes) =
-    Handle (toRealExp e) (MAP (\ (p,e). (p, toRealExp e)) pes) ∧
-  toRealExp (Con mod exps) = Con mod (MAP toRealExp exps) ∧
-  toRealExp (Fun s e) = Fun s (toRealExp e) ∧
-  toRealExp (App op exps) =
-    (let exps_real = MAP toRealExp exps in
+(* WAS: toRealExp : CakeML AST -> CakeML AST *)
+Definition realify_def:
+  realify (Lit (Word64 w)) = Lit (Word64 w) (* RealFromFP added in App case *)∧
+  realify (Lit l) = Lit l ∧
+  realify (Var x) = Var x ∧
+  realify (Raise e) = Raise (realify e) ∧
+  realify (Handle e pes) =
+    Handle (realify e) (MAP (\ (p,e). (p, realify e)) pes) ∧
+  realify (Con mod exps) = Con mod (MAP realify exps) ∧
+  realify (Fun s e) = Fun s (realify e) ∧
+  realify (App op exps) =
+    (let exps_real = MAP realify exps in
      case op of
      | FpFromWord => App  RealFromFP exps_real
      | FP_cmp cmp => App (Real_cmp (getRealCmp cmp)) exps_real
@@ -195,22 +184,22 @@ Definition toRealExp_def:
      | FP_top _ =>
      (case exps of
       | [e1; e2; e3] => App (Real_bop (Real_Add)) [
-                          App (Real_bop (Real_Mul)) [toRealExp e2; toRealExp e3]; toRealExp e1]
+                          App (Real_bop (Real_Mul)) [realify e2; realify e3]; realify e1]
       | _ => App op exps_real) (* malformed expression, return garbled output *)
      | _ => App op exps_real) ∧
-  toRealExp (Log lop e2 e3) =
-    Log lop (toRealExp e2) (toRealExp e3) ∧
-  toRealExp (If e1 e2 e3) =
-    If (toRealExp e1) (toRealExp e2) (toRealExp e3) ∧
-  toRealExp (Mat e pes) =
-    Mat (toRealExp e) (MAP (λ(p,e). (p, toRealExp e)) pes) ∧
-  toRealExp (Let so e1 e2) =
-    Let so (toRealExp e1) (toRealExp e2) ∧
-  toRealExp (Letrec ses e) =
-    Letrec (MAP (λ (s1,s2,e). (s1, s2, toRealExp e)) ses) (toRealExp e) ∧
-  toRealExp (Tannot e t) = Tannot (toRealExp e) t ∧
-  toRealExp (Lannot e l) = Lannot (toRealExp e) l ∧
-  toRealExp (FpOptimise sc e) = FpOptimise sc (toRealExp e)
+  realify (Log lop e2 e3) =
+    Log lop (realify e2) (realify e3) ∧
+  realify (If e1 e2 e3) =
+    If (realify e1) (realify e2) (realify e3) ∧
+  realify (Mat e pes) =
+    Mat (realify e) (MAP (λ(p,e). (p, realify e)) pes) ∧
+  realify (Let so e1 e2) =
+    Let so (realify e1) (realify e2) ∧
+  realify (Letrec ses e) =
+    Letrec (MAP (λ (s1,s2,e). (s1, s2, realify e)) ses) (realify e) ∧
+  realify (Tannot e t) = Tannot (realify e) t ∧
+  realify (Lannot e l) = Lannot (realify e) l ∧
+  realify (FpOptimise sc e) = FpOptimise sc (realify e)
 Termination
   wf_rel_tac ‘measure exp_size’ \\ fs[astTheory.exp_size_def] \\ rpt conj_tac
   >- (Induct_on `ses` \\ fs[astTheory.exp_size_def]
@@ -230,16 +219,188 @@ Termination
       \\ first_x_assum (qspec_then `mod'` assume_tac) \\ fs[])
 End
 
-Definition getFunctions_def:
-  getFunctions (Dletrec l funs) = SOME funs ∧
-  getFunctions _ = NONE
+Definition stripFuns_def:
+  stripFuns (Fun var body):(((string, string) id) list# ast$exp)=
+    (let (vars, body) = stripFuns body in
+    (Short var :: vars, body)) ∧
+  stripFuns e = ([], e)
 End
 
-Definition stripFuns_def:
-  stripFuns (Fun var body) =
-    (let (vars, body) = stripFuns body in
-    (var :: vars, body)) ∧
-  stripFuns e = ([], e)
+Definition freevars_list_def:
+  freevars_list [] = [] /\
+  freevars_list [ast$Var n] = [ n ] /\
+  freevars_list [Lit l] = [] /\
+  freevars_list [Raise e] = freevars_list [e] /\
+  freevars_list [Handle e pes] =
+    FOLDL (\ vars. \ (p,e). (freevars_list [e]) ++ vars) (freevars_list [e]) pes /\
+  freevars_list [Con id es] = freevars_list es /\
+  freevars_list [Fun s e] = FILTER (λ x. x ≠ Short s) (freevars_list [e]) /\
+  freevars_list [App op es] = freevars_list es /\
+  freevars_list [Log lop e1 e2] = (freevars_list [e1] ++ freevars_list [e2]) /\
+  freevars_list [If e1 e2 e3] = (freevars_list [e1] ++ freevars_list [e2] ++ freevars_list [e3]) /\
+  freevars_list [Mat e pes] =
+    FOLDL (\ vars. \ (p,e). (freevars_list [e]) ++ vars) (freevars_list [e]) pes /\
+  freevars_list [Let x e1 e2] =
+    freevars_list [e1] ++
+    (case x of
+     | NONE => freevars_list [e2]
+     | SOME s => FILTER (λ x. x ≠ Short s) (freevars_list [e2])) ∧
+  freevars_list [Letrec fs e] = [] (* TODO *) /\
+  freevars_list [Tannot e t] = freevars_list [e] /\
+  freevars_list [Lannot e l] = freevars_list [e] /\
+  freevars_list [FpOptimise opt e] = freevars_list [e] /\
+  freevars_list (e1::es) =
+    freevars_list [e1] ++ freevars_list es
+Termination
+  wf_rel_tac `measure exp6_size` \\ fs[]
+  \\ Induct_on `pes` \\ fs[]
+  \\ rpt strip_tac \\ simp[astTheory.exp_size_def]  \\ rveq
+  \\ res_tac
+  >- (simp[astTheory.exp_size_def])
+  \\ first_x_assum (qspec_then `e` assume_tac) \\ fs[]
+End
+
+Definition checkFreevars_def:
+  checkFreevars [] _ = T ∧
+  checkFreevars (x::xs) fVars = if (MEM x fVars) then checkFreevars xs fVars else F
+End
+
+Definition computeErrorbounds_def:
+  computeErrorbounds theCmd P Gamma =
+  let theCmd = toRCmd theCmd in
+    case inferIntervalboundsCmd theCmd P FloverMapTree_empty of
+    | NONE => NONE
+    | SOME theRealBounds =>
+    case getValidMapCmd Gamma theCmd FloverMapTree_empty of
+    | Fail _ => NONE
+    | FailDet _ _ => NONE
+    | Succes typeMap =>
+    case inferErrorboundCmd theCmd typeMap theRealBounds FloverMapTree_empty of
+    | NONE => NONE
+    | SOME theErrBounds =>
+    case (CertificateCheckerCmd theCmd theErrBounds P Gamma)
+    of SOME Gamma => SOME theErrBounds
+    | _ => NONE
+End
+
+Definition mkFloVerPre_def:
+  mkFloVerPre (P:(string,string) id -> (real#real)) (varMap:nameP list) =
+  λ n:num.
+  case lookupFloVerVar n varMap of
+  | NONE => (0,0)
+  | SOME (x,m) => P x
+End
+
+Definition getErrorbounds_def:
+  getErrorbounds decl P =
+  if (LENGTH decl ≠ 1) then (NONE, SOME "Only a single kernel is currently supported") else
+  case decl of
+  | [Dlet loc (Pvar p) e] =>
+    (let (vars, body) = stripFuns e in
+     case e of
+     |FpOptimise NoOpt e' =>
+     (case getFloVerVarMap vars of
+      | NONE =>
+      (NONE,
+       SOME "Could not build a valid variable map for kernel. Possibly due to double binding of variables")
+      | SOME (floverVars, varMap, freshId) =>
+      (* check that freevars and vars agree: *)
+      if (checkFreevars vars (freevars_list [body]))
+      then
+      let
+      Gamma = buildFloVerTypeMap floverVars;
+      in
+      case (toFloVerCmd varMap freshId body) of
+      | NONE => (NONE, SOME "Could not translate body to valid FloVer AST")
+      | SOME (theIds, freshId, theCmd) =>
+      case computeErrorbounds theCmd (mkFloVerPre P varMap) Gamma of
+      | SOME theBounds => (SOME (theBounds, theCmd, vars), NONE)
+      | NONE => (NONE, SOME "Could not compute or check roundoff errors for FloVer AST")
+      else (NONE,SOME "The free variables of the function body do not agree with the parameters specified"))
+     | _ => (NONE, SOME "Only Dlet is currently supported"))
+     | _ => (NONE, SOME "Body must start with NoOpt annotation")
+End
+
+Definition isOkError_def:
+  isOkError decl P (err:real) =
+  case getErrorbounds decl P of
+  | (NONE, err) => (NONE, err)
+  | (SOME (bounds, cmd, _), _) =>
+    case FloverMapTree_find (getRetExp (toRCmd cmd)) bounds of
+    | NONE => (NONE, SOME "Something went wrong internally. Please report this")
+    | SOME (iv,errD) => (SOME (errD ≤ err), NONE)
+End
+
+val _ = export_theory ();
+
+    (**
+Definition Eval_oracle_def:
+  Eval_oracle env exp P oracle =
+  ∀ refs.
+  ∃ res.
+End
+
+
+Theorem evaluate_const:
+  Eval env (App FpFromWord [Lit (Word64 w)]) ((=) (FP_WordTree (Fp_const w)))
+Proof
+  fs[ml_translatorTheory.Eval_def, ml_progTheory.eval_rel_def]
+  \\ EVAL_TAC \\ fs[]
+QED
+
+Theorem evaluate_var:
+  nsLookup env.v (Short x) = SOME fp ⇒
+  Eval env (Var (Short x)) ((=) fp)
+Proof
+  fs[ml_translatorTheory.Eval_def, ml_progTheory.eval_rel_def]
+  \\ EVAL_TAC \\ fs[]
+QED
+
+Theorem evaluate_bop:
+  Eval env e1 ((=) (FP_WordTree fp1)) ∧
+  Eval env e2 ((=) (FP_WordTree fp2)) ⇒
+  Eval env (App (FP_bop bop) [e1;e2]) ((=) (FP_WordTree (Fp_bop bop fpT1 fpT2)))
+Proof
+  rpt strip_tac
+  \\ simp [ml_translatorTheory.Eval_def, ml_progTheory.eval_rel_def]
+  \\ simp[terminationTheory.evaluate_def, astTheorsemanticPrimitivesTheoryy.getOpClass_def]
+  \\ EVAL_TAC \\ fs[]
+
+
+
+exception valError of string;
+
+fun translate t =
+  case free_vars t of
+  v::vs => raise valError "No free vars allowed"
+  | [] =>
+**)
+
+(** UNUSED:
+
+Definition isFloVerExps_def:
+  isFloVerExps [Var x] = T ∧
+  isFloVerExps [App op exps] =
+    (isFloVerExps exps  ∧
+    (case op of
+     | FP_bop _ => LENGTH exps = 2
+     | FP_uop FP_Neg => LENGTH exps = 1
+     | FP_top _ => LENGTH exps = 3
+     | _ =>  F)) ∧
+  isFloVerExps [e] = F ∧
+  isFloVerExps (e1::es) = (isFloVerExps [e1] ∧ isFloVerExps es)
+Termination
+  wf_rel_tac `measure exp6_size`
+End
+
+Definition isFloVerCmd_def:
+  isFloVerCmd (Let so e1 e2) =
+  (case so of
+   | SOME x => isFloVerExps [e1] ∧ isFloVerCmd e2
+   | NONE => F) ∧
+  isFloVerCmd (App op exps) = isFloVerExps [App op exps] ∧
+  isFloVerCmd (Var x) = T ∧
+  isFloVerCmd _ = F
 End
 
 Definition stripAssert_def:
@@ -251,11 +412,6 @@ Definition stripAssert_def:
       else NONE
     | _ => NONE) ∧
   stripAssert _ = NONE
-End
-
-Definition stripNoOpt_def:
-  stripNoOpt (FpOptimise NoOpt e) = e ∧
-  stripNoOpt e = e
 End
 
 Definition prepareKernel_def:
@@ -362,87 +518,4 @@ Definition toFloVerPre_def:
   toFloVerPre _ _ = NONE
 End
 
-Definition computeErrorbounds_def:
-  computeErrorbounds theCmd P Gamma =
-  let theCmd = toRCmd theCmd in
-    case inferIntervalboundsCmd theCmd P FloverMapTree_empty of
-    | NONE => NONE
-    | SOME theRealBounds =>
-    case getValidMapCmd Gamma theCmd FloverMapTree_empty of
-    | Fail _ => NONE
-    | FailDet _ _ => NONE
-    | Succes typeMap =>
-    case inferErrorboundCmd theCmd typeMap theRealBounds FloverMapTree_empty of
-    | NONE => NONE
-    | SOME theErrBounds =>
-    case (CertificateCheckerCmd theCmd theErrBounds P Gamma)
-    of SOME Gamma => SOME theErrBounds
-    | _ => NONE
-End
-
-Definition freevars_list_def:
-  freevars_list [] = [] /\
-  freevars_list [ast$Var n] = [ n ] /\
-  freevars_list [Lit l] = [] /\
-  freevars_list [Raise e] = freevars_list [e] /\
-  freevars_list [Handle e pes] =
-    FOLDL (\ vars. \ (p,e). (freevars_list [e]) ++ vars) (freevars_list [e]) pes /\
-  freevars_list [Con id es] = freevars_list es /\
-  freevars_list [Fun s e] = FILTER (λ x. x ≠ Short s) (freevars_list [e]) /\
-  freevars_list [App op es] = freevars_list es /\
-  freevars_list [Log lop e1 e2] = (freevars_list [e1] ++ freevars_list [e2]) /\
-  freevars_list [If e1 e2 e3] = (freevars_list [e1] ++ freevars_list [e2] ++ freevars_list [e3]) /\
-  freevars_list [Mat e pes] =
-    FOLDL (\ vars. \ (p,e). (freevars_list [e]) ++ vars) (freevars_list [e]) pes /\
-  freevars_list [Let x e1 e2] =
-    freevars_list [e1] ++
-    (case x of
-     | NONE => freevars_list [e2]
-     | SOME s => FILTER (λ x. x ≠ Short s) (freevars_list [e2])) ∧
-  freevars_list [Letrec fs e] = [] (* TODO *) /\
-  freevars_list [Tannot e t] = freevars_list [e] /\
-  freevars_list [Lannot e l] = freevars_list [e] /\
-  freevars_list [FpOptimise opt e] = freevars_list [e] /\
-  freevars_list (e1::es) =
-    freevars_list [e1] ++ freevars_list es
-Termination
-  wf_rel_tac `measure exp6_size` \\ fs[]
-  \\ Induct_on `pes` \\ fs[]
-  \\ rpt strip_tac \\ simp[astTheory.exp_size_def]  \\ rveq
-  \\ res_tac
-  >- (simp[astTheory.exp_size_def])
-  \\ first_x_assum (qspec_then `e` assume_tac) \\ fs[]
-End
-
-Definition checkFreevars_def:
-  checkFreevars [] _ = T ∧
-  checkFreevars (x::xs) fVars = if (MEM x fVars) then checkFreevars xs fVars else F
-End
-
-Definition getErrorbounds_def:
-  getErrorbounds decl =
-    case prepareKernel (getFunctions decl) of
-    | NONE => NONE
-    | SOME (ids, cake_P, f) =>
-    case prepareVars ids of
-    | NONE => NONE
-    | SOME (floverVars,varMap,freshId) =>
-    (* check that freevars and varMap agree: *)
-    if (checkFreevars (MAP FST varMap) (freevars_list [f]))
-    then
-      let
-        Gamma = prepareGamma floverVars;
-        in
-      case (toFloVerCmd varMap freshId f) of
-      | NONE => NONE
-      | SOME (theIds, freshId, theCmd) =>
-      case toFloVerPre [cake_P] varMap of
-      | NONE => NONE
-      | SOME (P,dVars) =>
-      case computeErrorbounds theCmd P Gamma of
-      | SOME theBounds => SOME (theBounds, theCmd)
-      | NONE => NONE
-    else NONE
-End
-
-val _ = export_theory ();
+**)
